rewrite small steps

plf/Smallstep.v
@@ -18,144 +18,280 @@ Fixpoint evalF (t : tm) : nat :=
   | P t1 t2 => evalF t1 + evalF t2
   end.
 
+Reserved Notation " t '==>' n " (at level 50, left associativity).
+
+Inductive eval : tm -> nat -> Prop :=
+  | E_Const : forall n,
+      C n ==> n
+  | E_Plus : forall t1 t2 n1 n2,
+      t1 ==> n1 ->
+      t2 ==> n2 ->
+      P t1 t2 ==> (n1 + n2)
+
+where " t '==>' n " := (eval t n).
+
+Module SimpleArith1.
+Reserved Notation " t '-->' t' " (at level 40).
+
 Inductive step : tm -> tm -> Prop :=
-| ST_PlusConstConst : forall n1 n2,
-    (step
-       (P (C n1) (C n2))
-       (C (n1 + n2)))
-| ST_Plus1 : forall t1 t1' t2,
-    (step t1 t1') -> (step (P t1 t2)
-                          (P t1' t2))
-| ST_Plus2 : forall n1 t2 t2',
-    (step t2 t2') -> (step (P (C n1) t2)
-                          (P (C n1) t2')).
+  | ST_PlusConstConst : forall n1 n2,
+      P (C n1) (C n2) --> C (n1 + n2)
+  | ST_Plus1 : forall t1 t1' t2,
+      t1 --> t1' ->
+      P t1 t2 --> P t1' t2
+  | ST_Plus2 : forall n1 t2 t2',
+      t2 --> t2' ->
+      P (C n1) t2 --> P (C n1) t2'
 
-Notation " t '-->' t' " := (step t t') (at level 50, left associativity).
-Example test_step_1 :
-      P
-        (P (C 1) (C 3))
-        (P (C 2) (C 4))
-      -->
-      P
-        (C 4)
-        (P (C 2) (C 4)).
-Proof.
-  apply ST_Plus1.
-  apply ST_PlusConstConst.
-Qed.
-
-Example test_step_2 :
-      P
-        (C 0)
-        (P
-          (C 2)
-          (P (C 1) (C 3)))
-      -->
-      P
-        (C 0)
-        (P
-          (C 2)
-          (C 4)).
-Proof.
-  apply ST_Plus2.
-  apply ST_Plus2.
-  apply ST_PlusConstConst.
-Qed.
-
+  where " t '-->' t' " := (step t t').
+End SimpleArith1.
 
 Definition relation (X : Type) := X -> X -> Prop.
+
+Definition deterministic {X : Type} (R : relation X) :=
+  forall x y1 y2 : X, R x y1 -> R x y2 -> y1 = y2.
+
+Module SimpleArith2.
+
+Import SimpleArith1.
+
+Theorem step_deterministic:
+  deterministic step.
+Proof.
+  unfold deterministic. intros x y1 y2 Hy1 Hy2.
+  generalize dependent y2.
+  induction Hy1; intros y2 Hy2.
+  - (* ST_PlusConstConst *) inversion Hy2; subst.
+    + (* ST_PlusConstConst *) reflexivity.
+    + (* ST_Plus1 *) inversion H2.
+    + (* ST_Plus2 *) inversion H2.
+  - (* ST_Plus1 *) inversion Hy2; subst.
+    + (* ST_PlusConstConst *)
+      inversion Hy1.
+    + (* ST_Plus1 *)
+      rewrite <- (IHHy1 t1'0).
+      reflexivity. assumption.
+    + (* ST_Plus2 *)
+      inversion Hy1.
+  - (* ST_Plus2 *) inversion Hy2; subst.
+    + (* ST_PlusConstConst *)
+      inversion Hy1.
+    + (* ST_Plus1 *) inversion H2.
+    + (* ST_Plus2 *)
+      rewrite <- (IHHy1 t2'0).
+      reflexivity. assumption.
+Qed.
+
+End SimpleArith2.
 
 Inductive value : tm -> Prop :=
   | v_const : forall n, value (C n).
 
-Module Temp4.
+Reserved Notation " t '-->' t' " (at level 40).
 
-  Inductive tm1 : Type :=
-  | tru : tm1
-  | fls : tm1
-  | test : tm1 -> tm1 -> tm1 -> tm1.
+Inductive step : tm -> tm -> Prop :=
+  | ST_PlusConstConst : forall n1 n2,
+          P (C n1) (C n2)
+      --> C (n1 + n2)
+  | ST_Plus1 : forall t1 t1' t2,
+        t1 --> t1' ->
+        P t1 t2 --> P t1' t2
+  | ST_Plus2 : forall v1 t2 t2',
+        value v1 ->                     (* <--- n.b. *)
+        t2 --> t2' ->
+        P v1 t2 --> P v1 t2'
 
-  Inductive value : tm1 -> Prop :=
-  | v_tru : value tru
-  | v_fls : value fls.
+  where " t '-->' t' " := (step t t').
 
-  Inductive step1 : tm1 -> tm1 -> Prop :=
-  | ST_IfTrue : forall t1 t2,
-      (step1 (test tru t1 t2)
-             t1)
-  | ST_IfFalse : forall t1 t2,
-      (step1 (test fls t1 t2)
-             t2)
-  | ST_If : forall t1 t1' t2 t3,
-      (step1 t1 t1') ->
-      (step1 (test t1 t2 t3)
-            (test t1' t2 t3)).
-  Notation " t '--->' t' " := (step1 t t') (at level 40).
+Theorem strong_progress : forall t,
+  value t \/ (exists t', t --> t').
+Proof.
+  induction t.
+  - (* C *) left. apply v_const.
+  - (* P *) right. destruct IHt1 as [IHt1 | [t1' Ht1] ].
+    + (* l *) destruct IHt2 as [IHt2 | [t2' Ht2] ].
+      * (* l *) inversion IHt1. inversion IHt2.
+        exists (C (n + n0)).
+        apply ST_PlusConstConst.
+      * (* r *)
+        exists (P t1 t2').
+        apply ST_Plus2. apply IHt1. apply Ht2.
+    + (* r *)
+      exists (P t1' t2).
+      apply ST_Plus1. apply Ht1.
+Qed.
 
-  Definition bool_step_propl :=
-    fls ---> fls.
+Definition normal_form {X : Type}
+              (R : relation X) (t : X) : Prop :=
+  ~ exists t', R t t'.
 
-End Temp4.
-
-(* Multi-Step Reduction *)
 Inductive multi {X : Type} (R : relation X) : relation X :=
-| multi_refl : forall (x : X), multi R x x
-| multi_step : forall (x y z : X), R x y -> multi R y z -> multi R x z.
+  | multi_refl : forall (x : X), multi R x x
+  | multi_step : forall (x y z : X),
+                    R x y ->
+                    multi R y z ->
+                    multi R x z.
 
 Notation " t '-->*' t' " := (multi step t t') (at level 40).
 
 Theorem multi_R : forall (X : Type) (R : relation X) (x y : X),
     R x y -> (multi R) x y.
 Proof.
-  intros.
-  apply multi_step with y.
-  apply H.
-  apply multi_refl.
+  intros X R x y H.
+  apply multi_step with y. apply H. apply multi_refl.
 Qed.
 
 Theorem multi_trans :
   forall (X : Type) (R : relation X) (x y z : X),
-    multi R x y -> multi R y z -> multi R x z.
+      multi R x y  ->
+      multi R y z ->
+      multi R x z.
 Proof.
-  intros.
+  intros X R x y z G H.
+  induction G.
+    - (* multi_refl *) assumption.
+    - (* multi_step *)
+      apply multi_step with y. assumption.
+      apply IHG. assumption.
+Qed.
+
+Definition step_normal_form := normal_form step.
+Definition normal_form_of (t t' : tm) :=
+  (t -->* t' /\ step_normal_form t').
+Definition normalizing {X : Type} (R : relation X) :=
+  forall t, exists t',
+    (multi R) t t' /\ normal_form R t'.
+Lemma multistep_congr_1 : forall t1 t1' t2,
+     t1 -->* t1' ->
+     P t1 t2 -->* P t1' t2.
+Proof.
+  intros t1 t1' t2 H. induction H.
+  - (* multi_refl *) apply multi_refl.
+  - (* multi_step *) apply multi_step with (P y t2).
+    + apply ST_Plus1. apply H.
+    + apply IHmulti.
+Qed.
+
+Check ST_Plus2.
+
+Theorem multistep_congr_2 : forall t1 t2 t2',
+  value t1 -> t2 -->* t2' -> P t1 t2 -->* P t1 t2'.
+Proof.
+  intros t1 t2 t2' Vt1 H.
   induction H.
-  - assumption.
-  - apply multi_step with y.
-    assumption.
-    apply IHmulti.
-    apply H0.
+  - constructor.
+  - apply multi_step with (P t1 y).
+    + apply ST_Plus2. easy. easy.
+    + assumption.
 Qed.
 
-Lemma test_multistep_1:
-      P
-        (P (C 0) (C 3))
-        (P (C 2) (C 4))
-   -->*
-      C ((0 + 3) + (2 + 4)).
+Lemma value_is_nf : forall v,
+  value v -> normal_form step v.
 Proof.
-  apply multi_step with
-      (P (C (0 + 3))
-         (P (C 2) (C 4))).
-  apply ST_Plus1.
-  apply ST_PlusConstConst.
-  apply multi_step with
-      (P (C (0 + 3))
-         (C (2 + 4))).
-  apply ST_Plus2.
-  apply ST_PlusConstConst.
-  apply multi_R.
-  apply ST_PlusConstConst.
+  unfold normal_form. intros v H. destruct H.
+  intros contra. destruct contra. inversion H.
 Qed.
 
-Inductive ev : nat -> Prop :=
-| ev_0 : ev 0
-| ev_SS : forall n, ev n -> ev (S (S n)).
+Lemma nf_is_value : forall t,
+  normal_form step t -> value t.
+Proof. (* a corollary of [strong_progress]... *)
+  unfold normal_form. intros t H.
+  assert (G : value t \/ exists t', t --> t').
+  { apply strong_progress. }
+  destruct G as [G | G].
+  - (* l *) apply G.
+  - (* r *) exfalso. apply H. assumption.
+Qed.
 
-Check ev_SS.
+Corollary nf_same_as_value : forall t,
+  normal_form step t <-> value t.
+Proof.
+  split. apply nf_is_value. apply value_is_nf.
+Qed.
 
-Check ev_SS 4 (ev_SS 2 (ev_SS 0 ev_0)).
+Theorem step_normalizing :
+  normalizing step.
+Proof.
+  unfold normalizing.
+  induction t.
+  - (* C *)
+    exists (C n).
+    split.
+    + (* l *) apply multi_refl.
+    + (* r *)
+      (* We can use [rewrite] with "iff" statements, not
+           just equalities: *)
+      rewrite nf_same_as_value. apply v_const.
+  - (* P *)
+    destruct IHt1 as [t1' [Hsteps1 Hnormal1] ].
+    destruct IHt2 as [t2' [Hsteps2 Hnormal2] ].
+    rewrite nf_same_as_value in Hnormal1.
+    rewrite nf_same_as_value in Hnormal2.
+    destruct Hnormal1 as [n1].
+    destruct Hnormal2 as [n2].
+    exists (C (n1 + n2)).
+    split.
+    + (* l *)
+      apply multi_trans with (P (C n1) t2).
+      * apply multistep_congr_1. apply Hsteps1.
+      * apply multi_trans with (P (C n1) (C n2)).
+        { apply multistep_congr_2. apply v_const. apply Hsteps2. }
+        apply multi_R. apply ST_PlusConstConst.
+    + (* r *)
+      rewrite nf_same_as_value. apply v_const.
+Qed.
 
+Theorem eval_multistep : forall t n,
+    t ==> n -> t -->* C n.
+Proof.
+  intros t n H.
+  induction H.
+  - constructor.
+  - apply multi_trans with (P (C n1) t2).
+    now apply multistep_congr_1.
+    apply multi_trans with (P (C n1) (C n2)).
+    now apply multistep_congr_2.
+    apply multi_step with (C (n1 + n2)).
+    apply ST_PlusConstConst.
+    apply multi_refl.
+Qed.
 
+Lemma step_eval : forall t t' n,
+    t --> t' ->
+    t' ==> n ->
+    t ==> n.
+Proof.
+  intros t t' n Hs.
+  generalize dependent n.
+  induction Hs; intros n Hn.
+  + inversion Hn.
+    apply E_Plus.
+    constructor.
+    constructor.
+  + inversion Hn.
+    subst.
+    apply IHHs in H1.
+    apply E_Plus; easy.
+  + inversion Hn.
+    subst.
+    apply IHHs in H4. apply E_Plus; easy.
+Qed.
+
+Theorem multistep_eval : forall t t',
+    normal_form_of t t' ->
+    exists n, t' = C n /\ t ==> n.
+Proof.
+  unfold normal_form_of, step_normal_form.
+  intros t t' [H1 H2].
+  apply nf_same_as_value in H2.
+  induction H1.
+  - inversion H2.
+    exists n. split. reflexivity. constructor.
+  - assert (exists n', z = C n' /\ y ==> n') as [n' [equal_z_Cn eval_y_n']].
+    apply IHmulti. assumption.
+    exists n'. split. assumption.
+    now apply step_eval with y.
+Qed.
 
 
 
