plf/Types.v
@@ -1,0 +1,65 @@
+Set Warnings "-notation-overridden,-parsing".
+From Coq Require Import Arith.Arith.
+From PLF Require Import Maps.
+From PLF Require Import Imp.
+From PLF Require Import Smallstep.
+Hint Constructors multi : core.
+
+Inductive tm : Type :=
+  | tru : tm
+  | fls : tm
+  | test : tm -> tm -> tm -> tm
+  | zro : tm
+  | scc : tm -> tm
+  | prd : tm -> tm
+  | iszro : tm -> tm.
+
+Inductive bvalue : tm -> Prop :=
+| bv_tru : bvalue tru
+| bv_fls : bvalue fls.
+
+Inductive nvalue : tm -> Prop :=
+| nv_zro : nvalue zro
+| nv_scc : forall t, nvalue t -> nvalue (scc t).
+
+Definition value (t : tm) := bvalue t \/ nvalue t.
+Hint Constructors bvalue nvalue : core.
+Hint Unfold value : core.
+
+Inductive step : tm -> tm -> Prop :=
+  | ST_TestTru : forall t1 t2,
+      (test tru t1 t2) --> t1
+  | ST_TestFls : forall t1 t2,
+      (test fls t1 t2) --> t2
+  | ST_Test : forall t1 t1' t2 t3,
+      t1 --> t1' ->
+      (test t1 t2 t3) --> (test t1' t2 t3)
+  | ST_Scc : forall t1 t1',
+      t1 --> t1' ->
+      (scc t1) --> (scc t1')
+  | ST_PrdZro :
+      (prd zro) --> zro
+  | ST_PrdScc : forall v,
+      nvalue v ->
+      (prd (scc v)) --> v
+  | ST_Prd : forall t1 t1',
+      t1 --> t1' ->
+      (prd t1) --> (prd t1')
+  | ST_IszroZro :
+      (iszro zro) --> tru
+  | ST_IszroScc : forall v,
+       nvalue v ->
+      (iszro (scc v)) --> fls
+  | ST_Iszro : forall t1 t1',
+      t1 --> t1' ->
+      (iszro t1) --> (iszro t1').
+
+Notation step_normal_form := (normal_form step).
+
+Definition stuck (t : tm) : Prop :=
+  step_normal_form t /\ ~ value t.
+
+Hint Unfold stuck : core.
+Example some_term_is_stuck :
+  exists t, stuck t.
+Proof.
